TypeEq -> TypeEqS

TabularTypeInterpreter/F⊗⊕ω/Lemmas/Type/Equivalence.lean
@@ -5,57 +5,422 @@ import TabularTypeInterpreter.«F⊗⊕ω».Lemmas.Type.ParallelReduction
 
 namespace TabularTypeInterpreter.«F⊗⊕ω»
 
-def TypeEquivalence.symm (h: [[Δ ⊢ A ≡ B]]): [[Δ ⊢ B ≡ A]] := by
+theorem ParallelReduction.TypeEquivalence_of (h: [[ Δ ⊢ A ≡> B ]]) (Alc: A.TypeVarLocallyClosed) : [[ Δ ⊢ A ≡ B ]] := by
   induction h with
-  | refl => exact .refl
-  | lamAppL => exact .lamAppR
-  | lamAppR => exact .lamAppL
-  | listAppL => exact .listAppR
-  | listAppR => exact .listAppL
-  | listAppIdL => exact .listAppIdR
-  | listAppIdR => exact .listAppIdL
-  | lam I h ih => exact .lam I ih
-  | app h₁ h₂ ih₁ ih₂ => exact .app ih₁ ih₂
-  | scheme I h ih => exact .scheme I ih
-  | arr h₁ h₂ ih₁ ih₂ => exact .arr ih₁ ih₂
-  | list h ih => exact .list ih
-  | listApp h₁ h₂ ih₁ ih₂ => exact .listApp ih₁ ih₂
-  | prod h ih => exact .prod ih
-  | sum h ih => exact .sum ih
-  | trans h₁ h₂ ih₁ ih₂ => exact .trans ih₂ ih₁
-
-theorem ParallelReduction.TypeEquivalence_of (h: [[ Δ ⊢ A ≡> B ]]) : [[ Δ ⊢ A ≡ B ]] := by
-  induction h with
-  | refl => exact .refl
-  | lamApp _ _ _ ih1 ih2 => exact .trans (.app (.lam _ ih1) ih2) .lamAppL
-  | lamListApp _ _ _ _ ih1 ih2 =>
+  | refl => exact (.refl Alc)
+  | lamApp _ AA' BB' ih1 ih2 =>
+    match Alc with
+    | .app (.lam Abody) Blc =>
+      simp_all [Abody.strengthen]
+      have A'body := Abody.modus_ponens_open (λ a nin => AA' a nin |>.preserve_lc)
+      have B'lc := BB'.preserve_lc Blc
+      exact .trans (.app (.lam _ ih1) ih2) (.lamApp A'body B'lc)
+  | lamListApp _ AA' BB' _ ih1 ih2 =>
+    match Alc with
+    | .listApp (.lam Abody) (.list Blc) =>
+      simp_all [Abody.strengthen, Std.Range.mem_toList_of_mem]
+      have A'body := Abody.modus_ponens_open (λ a nin => AA' a nin |>.preserve_lc)
+      have B'lc := λi itln => BB' i itln |>.preserve_lc (Blc i (Std.Range.mem_toList_of_mem itln))
       exact .trans (.listApp (.lam _ ih1) (.list ih2))
-                (.trans .listAppL (.list λx xin => .lamAppL))
-  | lam _ ih => exact .lam _ ih
-  | app _ _ ih1 ih2 => exact .app ih1 ih2
-  | scheme _ ih => exact .scheme _ ih
-  | arr _ _ ih1 ih2 => exact .arr ih1 ih2
-  | list _ ih => exact .list ih
-  | listApp _ _ ih1 ih2 => exact .listApp ih1 ih2
-  | prod _ ih => exact .prod ih
-  | sum _ ih => exact .sum ih
+                (.trans (.lamListApp A'body.lam B'lc) (.list λi iltn => (.lamApp A'body (B'lc i iltn))))
+  | lam _ ih =>
+    match Alc with | .lam Alc => have ih := λx nin => ih x nin Alc.strengthen; exact .lam _ ih
+  | app _ _ ih1 ih2 =>
+    match Alc with | .app Alc Blc => simp_all; exact .app ih1 ih2
+  | scheme _ ih =>
+    match Alc with | .forall Abody => simp_all [Abody.strengthen]; exact .scheme _ ih
+  | arr _ _ ih1 ih2 =>
+    match Alc with | .arr Alc Blc => simp_all; exact .arr ih1 ih2
+  | list _ ih =>
+    match Alc with | .list Alc => simp_all [Std.Range.mem_toList_of_mem]; exact .list ih
+  | listApp _ _ ih1 ih2 =>
+    match Alc with | .listApp Alc Blc => simp_all; exact .listApp ih1 ih2
+  | prod _ ih => match Alc with | .prod Alc => simp_all; exact .prod ih
+  | sum _ ih => match Alc with | .sum Alc => simp_all; exact .sum ih
 
-theorem EqParallelReduction.TypeEquivalence_of (h: [[ Δ ⊢ A <≡>* B ]]) : [[ Δ ⊢ A ≡ B ]] := by
+theorem EqParallelReduction.TypeEquivalence_of (h: [[ Δ ⊢ A <≡>* B ]]) (Alc: A.TypeVarLocallyClosed) : [[ Δ ⊢ A ≡ B ]] := by
   induction h with
-  | refl => exact .refl
-  | step h => exact h.TypeEquivalence_of
-  | sym BA ih => exact ih.symm
-  | trans AB BC ih1 ih2 => exact ih1.trans ih2
+  | refl => exact .refl Alc
+  | step h => exact h.TypeEquivalence_of Alc
+  | sym BA ih => exact ih (BA.preserve_lc.2 Alc) |>.symm
+  | trans AB BC ih1 ih2 => exact (ih1 Alc).trans (ih2 <| AB.preserve_lc.1 Alc)
+
+namespace TypeEquivalenceI
+
+local instance : Inhabited «Type» where
+  default := .list []
+in
+def list' (As Bs: List «Type») (length_eq: As.length = Bs.length) (h : ∀A B, ⟨A, B⟩ ∈ As.zip Bs → [[ Δ ⊢ A ≡ᵢ B ]] )
+  : TypeEquivalenceI Δ (.list As) (.list Bs) := by
+  rw [← Std.Range.map_get!_eq (as := As), ← Std.Range.map_get!_eq (as := Bs), ← length_eq]
+  apply list
+  intro i mem
+  apply h
+  have := (As.zip Bs).get!_mem <| by
+    rw [List.length_zip, ← length_eq, Nat.min_self]
+    exact mem.upper
+  rw [List.get!_zip length_eq mem.upper] at this
+  exact this
+
+theorem subst_rename' {a': TypeVarId}
+  (h: [[ Δ, a: K, Δ' ⊢ A ≡ᵢ B ]]):
+  [[ Δ, Δ'[a'/a] ⊢ A[a'/a] ≡ᵢ B[a'/a] ]] := by
+  have a'lc: [[ (a') ]].TypeVarLocallyClosed := by constructor
+  generalize Δ_eq: [[ (Δ, a: K, Δ') ]] = Δ_ at h
+  induction h generalizing Δ Δ' <;> (try simp_all [Type.TypeVar_subst]) <;> subst Δ_eq <;> try aesop (add unsafe constructors TypeEquivalenceI)
+  . case refl A lc => exact .refl (lc.TypeVar_subst a'lc)
+  . case lamApp A B K' Abody Blc =>
+    rw [a'lc.Type_open_TypeVar_subst_dist]
+    exact .lamApp (Abody.TypeVar_subst <| a'lc.weaken (n := 1)) (Blc.TypeVar_subst a'lc)
+  . case lamListApp A n B Alc Blc =>
+    unfold Function.comp
+    simp_all [Type.TypeVar_subst]
+    exact .lamListApp (Alc.TypeVar_subst a'lc) (λi iltn => Blc i iltn |>.TypeVar_subst a'lc)
+  . case listAppId A K' Alc => exact .listAppId (Alc.TypeVar_subst a'lc)
+  . case lam K' A B I AB ih =>
+    apply TypeEquivalenceI.lam (I := a :: I ++ Δ.typeVarDom ++ Δ'.typeVarDom)
+    intro a'' nin
+    repeat rw [<- a'lc.TypeVar_open_TypeVar_subst_comm (neq := by aesop)]
+    rw [Environment.append_typeExt_assoc, Environment.typeExt_subst]
+    apply ih <;> simp_all [Environment.append]
+  . case scheme K' A B I AB ih =>
+    apply TypeEquivalenceI.scheme (I := a :: I ++ Δ.typeVarDom ++ Δ'.typeVarDom)
+    intro a'' nin
+    repeat rw [<- a'lc.TypeVar_open_TypeVar_subst_comm (neq := by aesop)]
+    rw [Environment.append_typeExt_assoc, Environment.typeExt_subst]
+    apply ih <;> simp_all [Environment.append]
+  . case listAppComp A₀ A₁ B K A₀lc A₁body Blc =>
+    exact .listAppComp
+      (A₀lc.TypeVar_subst a'lc)
+      (A₁body.TypeVar_subst <| a'lc.weaken (n := 1))
+      (Blc.TypeVar_subst a'lc)
+
+theorem subst_rename {a': TypeVarId} (h: [[ Δ, a: K ⊢ A ≡ᵢ B ]]): [[ Δ ⊢ A[a'/a] ≡ᵢ B[a'/a] ]] :=
+  subst_rename' (Δ' := [[ ε ]]) h
+
+theorem weakening_type' (h: [[ Δ, Δ' ⊢ A ≡ᵢ B ]]) (fresh: a ∉ Δ.typeVarDom) : [[ Δ, a: K, Δ' ⊢ A ≡ᵢ B ]] := by
+  generalize Δ_eq : [[ (Δ, Δ') ]] = Δ_ at h
+  induction h generalizing Δ Δ' <;> subst Δ_eq <;> try aesop (add norm Type.freeTypeVars) (add unsafe constructors TypeEquivalenceI)
+  . case lam K' A B I AB ih =>
+    apply TypeEquivalenceI.lam (I := a :: I ++ Δ.typeVarDom)
+    intro a' nin
+    specialize @ih a' (by simp_all) Δ (Δ'.typeExt a' K')
+    simp_all [Environment.append]
+  . case scheme K' A B I AB ih =>
+    apply TypeEquivalenceI.scheme (I := a :: I ++ Δ.typeVarDom)
+    intro a' nin
+    specialize @ih a' (by simp_all) Δ (Δ'.typeExt a' K')
+    simp_all [Environment.append]
+
+theorem weakening_type (h: [[ Δ ⊢ A ≡ᵢ B ]]) (fresh: a ∉ Δ.typeVarDom) : [[ Δ, a: K ⊢ A ≡ᵢ B ]] := weakening_type' (Δ' := [[ ε ]]) h fresh
+
+theorem lam_intro_ex a (fresh: a ∉ A.freeTypeVars ++ B.freeTypeVars ++ Δ.typeVarDom) (h: [[ Δ, a : K ⊢ A^a ≡ᵢ B^a ]]): [[ Δ ⊢ (λ a : K. A) ≡ᵢ (λ a : K. B) ]] := by
+  refine .lam (I := a :: Δ.typeVarDom) ?_
+  intro a' notIn
+  repeat1' rw [Type.TypeVar_open_eq_Type_open_var]
+  repeat1' rw [<- Type.TypeVar_subst_intro_of_not_mem_freeTypeVars (a := a) (by simp_all)]
+  exact h.subst_rename.weakening_type (by simp_all)
+
+theorem scheme_intro_ex a (fresh: a ∉ A.freeTypeVars ++ B.freeTypeVars ++ Δ.typeVarDom) (h: [[ Δ, a : K ⊢ A^a ≡ᵢ B^a ]]): [[ Δ ⊢ (∀ a : K. A) ≡ᵢ (∀ a : K. B) ]] := by
+  refine .scheme (I := a :: Δ.typeVarDom) ?_
+  intro a' notIn
+  repeat1' rw [Type.TypeVar_open_eq_Type_open_var]
+  repeat1' rw [<- Type.TypeVar_subst_intro_of_not_mem_freeTypeVars (a := a) (by simp_all)]
+  exact h.subst_rename.weakening_type (by simp_all)
+
+open «Type» TypeVarLocallyClosed in
+theorem regularity (h: [[ Δ ⊢ A ≡ᵢ B ]]): A.TypeVarLocallyClosed ∧ B.TypeVarLocallyClosed := by
+  induction h
+  case lam Δ K A B I AB ih =>
+    have ⟨a, notIn⟩ := (I ++ A.freeTypeVars ++ B.freeTypeVars).exists_fresh
+    have ⟨Alc, Blc⟩ := ih a (by simp_all)
+    have Alc := Alc.TypeVar_close_inc (a := a); rw [TypeVar_close_TypeVar_open_eq_of_not_mem_freeTypeVars (by simp_all)] at Alc
+    have Blc := Blc.TypeVar_close_inc (a := a); rw [TypeVar_close_TypeVar_open_eq_of_not_mem_freeTypeVars (by simp_all)] at Blc
+    exact ⟨Alc.lam, Blc.lam⟩
+  case scheme Δ K A B I AB ih =>
+    have ⟨a, notIn⟩ := (I ++ A.freeTypeVars ++ B.freeTypeVars).exists_fresh
+    have ⟨Alc, Blc⟩ := ih a (by simp_all)
+    have Alc := Alc.TypeVar_close_inc (a := a); rw [TypeVar_close_TypeVar_open_eq_of_not_mem_freeTypeVars (by simp_all)] at Alc
+    have Blc := Blc.TypeVar_close_inc (a := a); rw [TypeVar_close_TypeVar_open_eq_of_not_mem_freeTypeVars (by simp_all)] at Blc
+    exact ⟨Alc.forall, Blc.forall⟩
+  case listAppComp A₀ A₁ B Δ K A₀lc A₁body Blc =>
+    exact ⟨A₀lc.listApp <| A₁body.lam.listApp Blc,  A₀lc.weaken (n:=1) |>.app A₁body |>.lam |>.listApp Blc⟩
+  all_goals aesop (add safe constructors TypeVarLocallyClosed, safe TypeVarLocallyClosed.weaken, safe forward Type_open_dec, safe forward Std.Range.mem_of_mem_toList)
+
+end TypeEquivalenceI
+
+namespace TypeEquivalenceS
+
+theorem sym (h: [[ Δ ⊢ A ≡ₛ B ]]) : [[ Δ ⊢ B ≡ₛ A ]] := by
+  induction h with
+  | base h => exact .symm h
+  | symm h => exact .base h
+  | trans _ _ ih1 ih2 => exact ih2.trans ih1
+
+theorem regularity (h: [[ Δ ⊢ A ≡ₛ B ]]): A.TypeVarLocallyClosed ∧ B.TypeVarLocallyClosed := by
+  induction h with
+  | base h => exact h.regularity
+  | symm h => exact ⟨h.regularity.2, h.regularity.1⟩
+  | trans _ _ ih1 ih2 => simp_all
+
+theorem lam_intro_ex a (fresh: a ∉ A.freeTypeVars ++ B.freeTypeVars ++ Δ.typeVarDom) (h: [[ Δ, a : K ⊢ A^a ≡ₛ B^a ]]): [[ Δ ⊢ (λ a : K. A) ≡ₛ (λ a : K. B) ]] := by
+  generalize Aa_eq : [[ (A^a) ]] = Aa at h
+  generalize Ba_eq : [[ (B^a) ]] = Ba at h
+  induction h generalizing A B
+  . case base h =>
+    subst Aa_eq Ba_eq
+    exact .base (TypeEquivalenceI.lam_intro_ex a fresh h)
+  . case symm h =>
+    subst Aa_eq Ba_eq
+    exact .symm (TypeEquivalenceI.lam_intro_ex a (by simp_all) h)
+  . case trans A_ B_ C_ AB BC ih1 ih2 =>
+    subst Aa_eq Ba_eq
+    have ⟨_, Blc⟩ := AB.regularity
+    specialize ih1 (B := [[\a^B_]]) (by simp_all [Type.not_mem_freeTypeVars_TypeVar_close]) rfl (by rw [Type.TypeVarLocallyClosed.TypeVar_open_TypeVar_close_id Blc])
+    specialize ih2 (A := [[\a^B_]]) (by simp_all [Type.not_mem_freeTypeVars_TypeVar_close]) (by rw [Type.TypeVarLocallyClosed.TypeVar_open_TypeVar_close_id Blc]) rfl
+    exact .trans ih1 ih2
+
+theorem scheme_intro_ex a (fresh: a ∉ A.freeTypeVars ++ B.freeTypeVars ++ Δ.typeVarDom) (h: [[ Δ, a : K ⊢ A^a ≡ₛ B^a ]]): [[ Δ ⊢ (∀ a : K. A) ≡ₛ (∀ a : K. B) ]] := by
+  generalize Aa_eq : [[ (A^a) ]] = Aa at h
+  generalize Ba_eq : [[ (B^a) ]] = Ba at h
+  induction h generalizing A B
+  . case base h =>
+    subst Aa_eq Ba_eq
+    exact .base (TypeEquivalenceI.scheme_intro_ex a fresh h)
+  . case symm h =>
+    subst Aa_eq Ba_eq
+    exact .symm (TypeEquivalenceI.scheme_intro_ex a (by simp_all) h)
+  . case trans A_ B_ C_ AB BC ih1 ih2 =>
+    subst Aa_eq Ba_eq
+    have ⟨_, Blc⟩ := AB.regularity
+    specialize ih1 (B := [[\a^B_]]) (by simp_all [Type.not_mem_freeTypeVars_TypeVar_close]) rfl (by rw [Type.TypeVarLocallyClosed.TypeVar_open_TypeVar_close_id Blc])
+    specialize ih2 (A := [[\a^B_]]) (by simp_all [Type.not_mem_freeTypeVars_TypeVar_close]) (by rw [Type.TypeVarLocallyClosed.TypeVar_open_TypeVar_close_id Blc]) rfl
+    exact .trans ih1 ih2
+
+private
+theorem ctor1 {T: «Type» → «Type»} (h: [[ Δ ⊢ A ≡ₛ B ]]) (c: ∀{Δ A B}, [[ Δ ⊢ A ≡ᵢ B]] → TypeEquivalenceI Δ (T A) (T B) ) : TypeEquivalenceS Δ (T A) (T B) := by
+  induction h with
+  | base h => exact .base (c h)
+  | symm h => exact .symm (c h)
+  | trans _ _ ih1 ih2 => exact ih1.trans ih2
+
+theorem prod (h: [[ Δ ⊢ A ≡ₛ B ]]) : [[ Δ ⊢ ⊗ A ≡ₛ ⊗ B ]] := ctor1 h (.prod)
+theorem sum (h: [[ Δ ⊢ A ≡ₛ B ]]) : [[ Δ ⊢ ⊕ A ≡ₛ ⊕ B ]] := ctor1 h (.sum)
+
+private
+theorem ctor2_left_refl {T: «Type» → «Type» → «Type»} (h: [[ Δ ⊢ A ≡ₛ A' ]]) (Clc: C.TypeVarLocallyClosed) (c: ∀{Δ A A' B B'}, [[ Δ ⊢ A ≡ᵢ A' ]] → [[ Δ ⊢ B ≡ᵢ B' ]] → TypeEquivalenceI Δ (T A B) (T A' B') ) : TypeEquivalenceS Δ (T C A) (T C A') := by
+  induction h with
+  | base h => exact .base (c (.refl Clc) h)
+  | symm h => exact .symm (c (.refl Clc) h)
+  | trans _ _ ih1 ih2 => exact ih1.trans ih2
+
+private
+theorem ctor2 {T: «Type» → «Type» → «Type»} (h1: [[ Δ ⊢ A ≡ₛ A' ]]) (h2: [[ Δ ⊢ B ≡ₛ B' ]]) (c: ∀{Δ A A' B B'}, [[ Δ ⊢ A ≡ᵢ A' ]] → [[ Δ ⊢ B ≡ᵢ B' ]] → TypeEquivalenceI Δ (T A B) (T A' B') ) : TypeEquivalenceS Δ (T A B) (T A' B') := by
+  induction h1 <;> induction h2
+  . case base.base h1 _ _ h2 => exact .base (c h1 h2)
+  . case base.symm h1 _ _ h2 =>
+    exact .trans
+      (.symm (c (.refl h1.regularity.1) h2))
+      (.base (c h1 (.refl h2.regularity.1)))
+  . case base.trans h _ _ _ _ BC ih1 ih2 =>
+    refine (.trans (.trans
+      ih1
+      (.symm (c h (.refl BC.regularity.1))))
+      ih2)
+  . case symm.base h1 _ _ h2 =>
+    exact .trans
+      (.base (c (.refl h1.regularity.2) h2))
+      (.symm (c h1 (.refl h2.regularity.2)))
+  . case symm.symm h1 _ _ h2 =>
+    exact .trans
+      (.symm (c (.refl h1.regularity.2) h2))
+      (.symm (c h1 (.refl h2.regularity.1)))
+  . case symm.trans h _ _ _ _ BC ih1 ih2 =>
+    exact (.trans (.trans
+      ih1
+      (.base (c h (.refl BC.regularity.1))))
+      ih2)
+  . case trans.base BC _ _ h ih1 ih2 =>
+    exact (.trans (.trans
+      ih1
+      (.symm (c (.refl BC.regularity.1) h)))
+      ih2)
+  . case trans.symm BC _ _ h ih1 ih2 =>
+    exact (.trans (.trans
+      ih1
+      (.base (c (.refl BC.regularity.1) h)))
+      ih2)
+  . case trans.trans A T A' AT TA' B U B' BU UB' _ _ ih1 ih2 =>
+    exact .trans (.trans
+      ih1
+      (ctor2_left_refl (BU.trans UB').sym AT.regularity.2 c))
+      ih2
+
+theorem app (h1: [[ Δ ⊢ A ≡ₛ A' ]]) (h2: [[ Δ ⊢ B ≡ₛ B' ]]) : [[ Δ ⊢ A B ≡ₛ A' B' ]] := ctor2 h1 h2 (.app)
+theorem arr (h1: [[ Δ ⊢ A ≡ₛ A' ]]) (h2: [[ Δ ⊢ B ≡ₛ B' ]]) : [[ Δ ⊢ A → B ≡ₛ A' → B' ]] := ctor2 h1 h2 (.arr)
+theorem listApp (h1: [[ Δ ⊢ A ≡ₛ A' ]]) (h2: [[ Δ ⊢ B ≡ₛ B' ]]) : [[ Δ ⊢ A ⟦B⟧ ≡ₛ A' ⟦B'⟧ ]] := ctor2 h1 h2 (.listApp)
+
+end TypeEquivalenceS
+
+-- TODO use upstream version after we upgrade to latest lott
+theorem _root_.Std.Range.mem_zip_map_append_cons {f g : Nat → α}
+  (h : xy ∈ (([:m - (i + 1)].map f) ++ x :: [m - i:m].map g).zip (([:m - (i + 1)].map f) ++ y :: [m - i:m].map g))
+  : (∃ j < m - (i + 1), xy.fst = f j ∧ xy.snd = f j) ∨
+    (xy.fst = x ∧ xy.snd = y) ∨
+    (∃ j, m - (i + 1) < j ∧ j < m ∧ xy.fst = g j ∧ xy.snd = g j) := sorry
+
+open Std.Range in
+theorem _root_.Std.Range.map_eq_cons_of_lt (mltn : m < n) : [m:n].map f = f m :: [m+1:n].map f := by
+  rw [map, toList, if_pos mltn, List.map_cons, ← map]
+
+open Std.Range in
+theorem _root_.Std.Range.map_same_eq_nil : [n:n].map f = [] := by
+  rw [map, toList, if_neg <| Nat.not_lt_of_le Nat.le.refl, List.map_nil]
+
+open Std.Range in
+theorem _root_.Std.Range.map_eq_snoc_of_lt (mltn : m < n) : [m:n].map f = [m:n - 1].map f ++ [f (n - 1)] := by
+  let npos := Nat.lt_of_le_of_lt (Nat.zero_le _) mltn
+  rw [map, ← map_append (l := m) (m := n - 1) (n := n) (Nat.le_sub_one_of_lt mltn) (Nat.sub_le _ _),
+      ← map, ← map, map_eq_cons_of_lt <| Nat.sub_lt npos Nat.one_pos, Nat.sub_add_cancel npos,
+      map_same_eq_nil]
 
 namespace TypeEquivalence
+
+theorem TypeEquivalenceS_of (h: [[Δ ⊢ A ≡ B]]) : [[Δ ⊢ A ≡ₛ B]] := by
+  induction h
+  . case refl lc => exact .base (.refl lc)
+  . case lamApp Abody Blc => exact .base (.lamApp Abody Blc)
+  . case lamListApp Alc Blc => exact .base (.lamListApp Alc Blc)
+  . case listAppId Alc => exact .base (.listAppId Alc)
+  . case lam Δ K A B I h ih =>
+    have ⟨a, nin⟩ := I ++ Δ.typeVarDom ++ A.freeTypeVars ++ B.freeTypeVars |>.exists_fresh
+    specialize ih a (by simp_all)
+    clear h
+    generalize Aa_eq: [[ (A^a) ]] = Aa at ih
+    generalize Ba_eq: [[ (B^a) ]] = Ba at ih
+    generalize Δ_eq : [[(Δ, a:K)]] = Δ_ at ih
+    induction ih generalizing A B Δ
+    . case base h =>
+      subst Aa_eq Ba_eq Δ_eq
+      refine TypeEquivalenceS.lam_intro_ex a (by simp_all) (.base h)
+    . case symm h =>
+      subst Aa_eq Ba_eq Δ_eq
+      refine TypeEquivalenceS.lam_intro_ex a (by simp_all) (.symm h)
+    . case trans A_ B_ C_ AB _ ih1 ih2 =>
+      have ⟨_, Blc⟩ := AB.regularity
+      subst Aa_eq Ba_eq Δ_eq
+      specialize ih1 (B := [[\a^B_]]) (by simp_all; exact Type.not_mem_freeTypeVars_TypeVar_close) rfl (by rw [Type.TypeVarLocallyClosed.TypeVar_open_TypeVar_close_id Blc]) rfl
+      specialize ih2 (A := [[\a^B_]]) (by simp_all; exact Type.not_mem_freeTypeVars_TypeVar_close) (by rw [Type.TypeVarLocallyClosed.TypeVar_open_TypeVar_close_id Blc]) rfl rfl
+      exact .trans ih1 ih2
+  . case app A1 A2 B1 B2 h1 h2 ih1 ih2 => exact ih1.app ih2
+  . case scheme Δ K A B I h ih =>
+    have ⟨a, nin⟩ := I ++ Δ.typeVarDom ++ A.freeTypeVars ++ B.freeTypeVars |>.exists_fresh
+    specialize ih a (by simp_all)
+    clear h
+    generalize Aa_eq: [[ (A^a) ]] = Aa at ih
+    generalize Ba_eq: [[ (B^a) ]] = Ba at ih
+    generalize Δ_eq : [[(Δ, a:K)]] = Δ_ at ih
+    induction ih generalizing A B Δ
+    . case base h =>
+      subst Aa_eq Ba_eq Δ_eq
+      refine TypeEquivalenceS.scheme_intro_ex a (by simp_all) (.base h)
+    . case symm h =>
+      subst Aa_eq Ba_eq Δ_eq
+      refine TypeEquivalenceS.scheme_intro_ex a (by simp_all) (.symm h)
+    . case trans A_ B_ C_ AB _ ih1 ih2 =>
+      have ⟨_, Blc⟩ := AB.regularity
+      subst Aa_eq Ba_eq Δ_eq
+      specialize ih1 (B := [[\a^B_]]) (by simp_all; exact Type.not_mem_freeTypeVars_TypeVar_close) rfl (by rw [Type.TypeVarLocallyClosed.TypeVar_open_TypeVar_close_id Blc]) rfl
+      specialize ih2 (A := [[\a^B_]]) (by simp_all; exact Type.not_mem_freeTypeVars_TypeVar_close) (by rw [Type.TypeVarLocallyClosed.TypeVar_open_TypeVar_close_id Blc]) rfl rfl
+      exact .trans ih1 ih2
+  . case arr ih1 ih2 => exact ih1.arr ih2
+  . case list n Δ A B h ih =>
+    clear h
+    have : ([:n].map fun i => B i) = ([:n - n].map fun i => A i) ++ [n - n:n].map fun i => B i := by
+      have : ([:0].map fun i => A i) = [] := by
+        rw [Std.Range.map, Std.Range.toList, if_neg nofun, List.map_nil]
+      rw [Nat.sub_self, this, List.nil_append]
+    rw [this]
+    generalize neqm : n = m
+    let nlem := Nat.le_refl n
+    rw (occs := .pos [3, 5]) [← neqm]
+    rw [neqm] at ih
+    rw (occs := .pos [2]) [neqm] at nlem
+    clear neqm this
+    induction n with
+    | zero =>
+      rw [Nat.sub_zero]
+      rw (occs := .pos [3]) [Std.Range.map]
+      rw [Std.Range.toList, if_neg (Nat.not_lt_of_le Nat.le.refl), List.map_nil, List.append_nil]
+      refine .base <| .refl ?_
+      . refine .list (λAi mem => ?_)
+        have ⟨i, iltm, eq⟩ := Std.Range.mem_of_mem_map mem; subst eq
+        exact ih i iltm |>.regularity.1
+    | succ i ih' =>
+      generalize A'eq : A (m - (i + 1)) = A', B'eq : B (m - (i + 1)) = B' at *
+      let ih'' := ih (m - (i + 1)) (by simp_all [Membership.mem]; omega)
+      specialize ih' <| Nat.le_of_add_right_le nlem
+      rw [A'eq, B'eq] at ih''
+      rw [Std.Range.map, ← Std.Range.map_append (Nat.zero_le _) (Nat.sub_le _ i),
+          ← Std.Range.map, ← Std.Range.map, Std.Range.map_eq_snoc_of_lt (by omega), Nat.sub_sub,
+          List.append_assoc, List.singleton_append, A'eq] at ih' ⊢
+      rw [List.append_assoc, List.singleton_append] at ih'
+      rw (occs := .pos [4]) [Std.Range.map_eq_cons_of_lt (by omega)]
+      rw [B'eq]
+      rw (occs := .pos [3]) [Nat.sub_add_eq]
+      rw [Nat.sub_add_cancel (by omega)]
+      clear A'eq B'eq
+      apply TypeEquivalenceS.trans ih'
+      clear ih'
+      induction ih'' with
+      | base h =>
+        refine .base <| .list' _ _ (by simp_all) (λ _ _ mem => ?_)
+        match Std.Range.mem_zip_map_append_cons mem with
+        | .inl ⟨j, jlt, Aeq, Beq⟩ =>
+          subst Aeq Beq
+          refine .refl ?_
+          . exact ih j (by simp_all [Membership.mem]; omega) |>.regularity.1
+        | .inr (.inl ⟨Aeq, Beq⟩) =>
+          subst Aeq Beq
+          exact h
+        | .inr (.inr ⟨j, ltj, jlt, Aeq, Beq⟩) =>
+          subst Aeq Beq
+          refine .refl ?_
+          . exact ih j (by simp_all [Membership.mem]; omega) |>.regularity.2
+      | symm h =>
+        refine .symm <| .list' _ _ (by simp_all) (λ _ _ mem => ?_)
+        match Std.Range.mem_zip_map_append_cons mem with
+        | .inl ⟨j, jlt, Aeq, Beq⟩ =>
+          subst Aeq Beq
+          refine .refl ?_
+          . exact ih j (by simp_all [Membership.mem]; omega) |>.regularity.1
+        | .inr (.inl ⟨Aeq, Beq⟩) =>
+          subst Aeq Beq
+          exact h
+        | .inr (.inr ⟨j, ltj, jlt, Aeq, Beq⟩) =>
+          subst Aeq Beq
+          refine .refl ?_
+          . exact ih j (by simp_all [Membership.mem]; omega) |>.regularity.2
+      | trans h h' ih'' ih''' =>
+        exact .trans ih'' ih'''
+  . case listApp ih1 ih2 => exact ih1.listApp ih2
+  . case listAppComp A₀lc A₁body Blc => exact .base (.listAppComp A₀lc A₁body Blc)
+  . case prod Δ A B h ih => exact ih.prod
+  . case sum ih => exact ih.sum
+  . case symm _ _ _ _ ih =>  exact ih.sym
+  . case trans _ _ _ _ _ _ ih1 ih2 => exact ih1.trans ih2
 
 theorem EqParallelReduction_of (eq: [[Δ ⊢ A ≡ B]]) : [[Δ ⊢ A <≡>* B]] := sorry
 
 theorem weakening (equiv: [[ Δ, Δ'' ⊢ A ≡ B ]]) (wfτ: [[ ⊢τ Δ, Δ', Δ'' ]]) : [[ Δ, Δ', Δ'' ⊢ A ≡ B ]] :=
-  equiv.EqParallelReduction_of |>.weakening wfτ |>.TypeEquivalence_of
+  -- equiv.EqParallelReduction_of |>.weakening wfτ |>.TypeEquivalence_of
+  -- TODO add lc precondition
+  sorry
 
 theorem subst' {A T T' : «Type»} (equiv : [[ Δ, a: K, Δ' ⊢ T ≡ T' ]]) (wf: [[ ⊢ Δ, a: K, Δ' ]]) (kindA: [[ Δ ⊢ A: K ]]) : [[ Δ, Δ'[A/a] ⊢ T[A/a] ≡ T'[A/a] ]] :=
-  equiv.EqParallelReduction_of |>.subst_out' wf kindA |>.TypeEquivalence_of
+  -- equiv.EqParallelReduction_of |>.subst_out' wf kindA |>.TypeEquivalence_of
+  -- TODO add lc precondition
+  sorry
 
 -- TODO this is not dt so properties on typing apparently have nothing to do with terms in env
 theorem TermVar_drop (equiv: [[ Δ, x: T, Δ'' ⊢ A ≡ B ]]): [[ Δ, Δ'' ⊢ A ≡ B ]] := sorry
